wip

src/ml/Pulse_RuntimeUtils.ml
@@ -182,7 +182,6 @@ let lax_check_term_with_unknown_universes (g:TcEnv.env) (e:S.term)
 
 let tc_term_phase1 (g:TcEnv.env) (e:S.term) (must_tot:bool) =
   let issues, res = FStarC_Errors.catch_errors (fun _ ->
-    let open FStarC_Tactics_V2_Basic in
     let g = TcEnv.set_range g e.pos in
     let g = {g with phase1=true; admit=true} in
     let e, t, guard = g.typeof_tot_or_gtot_term g e must_tot in
